---
title: "Find the roots of the quadratic equation x^2 - 4x + 4 = 0"
summary: "The roots of x^2 - 4x + 4 = 0 are both x = 2."
author: "Dr. Michael Green"
degree: "PhD in Condensed Matter Physics, University of Bristol"
tutor_type: "A-Level Maths Tutor"
date: 2024-04-09
---

The roots of the equation $x^2 - 4x + 4 = 0$ are both $x = 2$.

To determine the roots of a quadratic equation in the standard form $ax^2 + bx + c = 0$, we can apply the quadratic formula:

$$
x = \frac{-b \pm \sqrt{b^2 - 4ac}}{2a}
$$

In this specific case, we have $a = 1$, $b = -4$, and $c = 4$. By substituting these values into the quadratic formula, we proceed as follows:

$$
x = \frac{-(-4) \pm \sqrt{(-4)^2 - 4(1)(4)}}{2(1)}
$$

This simplifies to:

$$
x = \frac{4 \pm \sqrt{16 - 16}}{2}
$$

Continuing the simplification, we find:

$$
x = \frac{4 \pm 0}{2}
$$

Thus, we obtain:

$$
x = 2
$$

Consequently, the equation $x^2 - 4x + 4 = 0$ has both roots equal to $x = 2$. 

To verify this result, we can also factor the quadratic equation:

$$
x^2 - 4x + 4 = (x - 2)(x - 2)
$$

Since both factors are identical, it confirms that the only solution is indeed $x = 2$.
    