---
title: "Differentiate the function y = tan(x)"
summary: "The derivative of the function y = tan(x) is sec^2(x), indicating the rate of change of the tangent function with respect to the variable x."
author: "Dr. Sarah Wilson"
degree: "MSc in Physics, University College London"
tutor_type: "A-Level Physics Tutor"
date: 2024-07-17
---

Let's enhance the content for clarity and readability while maintaining the mathematical formatting.

---

The derivative of the function \( y = \tan(x) \) is given by \( \sec^2(x) \).

To differentiate \( y = \tan(x) \), we can apply the quotient rule. We start by expressing \( y \) as a quotient: let \( u = \sin(x) \) and \( v = \cos(x) \). Thus, we can rewrite \( y \) as:

$$
y = \frac{u}{v}
$$

According to the quotient rule, the derivative \( y' \) can be calculated using the formula:

$$
y' = \frac{v \cdot u' - u \cdot v'}{v^2}
$$

In this case, we have \( u' = \cos(x) \) (the derivative of \( \sin(x) \)) and \( v' = -\sin(x) \) (the derivative of \( \cos(x) \)). Substituting these derivatives into the quotient rule gives us:

$$
y' = \frac{\cos(x) \cdot \cos(x) - \sin(x) \cdot (-\sin(x))}{\cos^2(x)}
$$

Now, simplifying the expression, we obtain:

$$
y' = \frac{\cos^2(x) + \sin^2(x)}{\cos^2(x)}
$$

Using the Pythagorean identity \( \cos^2(x) + \sin^2(x) = 1 \), we can further simplify this to:

$$
y' = \frac{1}{\cos^2(x)}
$$

Since we know that \( \sec(x) = \frac{1}{\cos(x)} \), we can express the derivative as:

$$
y' = \sec^2(x)
$$

In conclusion, the derivative of \( y = \tan(x) \) is indeed \( \sec^2(x) \).
    