---
title: "How to derive the formulas for hyperbolic cosecant?"
summary: "How to derive the formulas for hyperbolic cosecant?"
author: "Dr. Daniel Thompson"
degree: "PhD in Relativity, University of Sheffield"
tutor_type: "A-Level Maths Tutor"
date: 2024-01-29
---

### Deriving the Formulas for Hyperbolic Cosecant

The hyperbolic cosecant function, denoted as $\text{csch}(x)$, is defined by the relationship:

$$
\text{csch}(x) = \frac{1}{\sinh(x)}.
$$

To derive its various formulas, we must begin with the definitions of the hyperbolic sine and cosine functions. 

Recall the definitions:

$$
\sinh(x) = \frac{e^x - e^{-x}}{2}
$$ 

and 

$$
\cosh(x) = \frac{e^x + e^{-x}}{2}.
$$ 

Using the definition of $\sinh(x)$, we can express $\text{csch}(x)$ as:

$$
\text{csch}(x) = \frac{1}{\sinh(x)} = \frac{2}{e^x - e^{-x}}.
$$

To simplify this expression further, we can multiply both the numerator and the denominator by $e^x$. This yields:

$$
\text{csch}(x) = \frac{2 e^x}{e^{2x} - 1}.
$$

Alternatively, we can express $\text{csch}(x)$ in another form:

$$
\text{csch}(x) = -\frac{2 e^{-x}}{1 - e^{-2x}}.
$$

With these formulas in hand, we can proceed to find the derivative of $\text{csch}(x)$ with respect to $x$. By applying the quotient rule, we have:

$$
\frac{d}{dx} \text{csch}(x) = -\frac{2 e^{-x}}{(1 - e^{-2x})^2} \cdot (-2 e^{-x}) = \frac{2 e^{-2x}}{(1 - e^{-2x})^2}.
$$

This simplifies to:

$$
\frac{d}{dx} \text{csch}(x) = 2 \text{csch}(x) \text{coth}(x).
$$

Next, we can find the integral of $\text{csch}(x)$ with respect to $x$. Using the substitution $u = e^x$, which leads to $du = e^x dx$, we can rewrite the integral as follows:

$$
\int \text{csch}(x) \, dx = \int \frac{1}{u} \cdot \frac{1}{1 - u^2} \, du.
$$

This integral can be evaluated as:

$$
\int \text{csch}(x) \, dx = -\frac{1}{2} \ln \left| \frac{u - 1}{u + 1} \right| + C = -\frac{1}{2} \ln \left| \frac{e^x - 1}{e^x + 1} \right| + C.
$$

In summary, the key formulas for the hyperbolic cosecant function are:

1. The hyperbolic cosecant function:
   $$
   \text{csch}(x) = \frac{2}{e^x - e^{-x}} = -\frac{2 e^{-x}}{1 - e^{-2x}}.
   $$

2. The derivative of hyperbolic cosecant:
   $$
   \frac{d}{dx} \text{csch}(x) = 2 \text{csch}(x) \text{coth}(x).
   $$

3. The integral of hyperbolic cosecant:
   $$
   \int \text{csch}(x) \, dx = -\frac{1}{2} \ln \left| \frac{e^x - 1}{e^x + 1} \right| + C.
   $$

These formulas provide a comprehensive understanding of the hyperbolic cosecant, its differentiation, and integration.
    