---
title: "Find the roots of the quadratic equation 2x^2 - 3x - 5 = 0"
summary: "To find the roots of the quadratic equation 2x^2 - 3x - 5 = 0, one can apply the quadratic formula or factorization methods."
author: "Prof. Peter Brown"
degree: "PhD in Mathematics, University of Warwick"
tutor_type: "IB Maths Tutor"
date: 2024-08-14
---

To find the roots of the quadratic equation 

$$
2x^2 - 3x - 5 = 0,
$$ 

we can utilize the quadratic formula, which is given by 

$$
x = \frac{-b \pm \sqrt{b^2 - 4ac}}{2a}.
$$ 

In this formula, the coefficients are defined as follows: $a = 2$, $b = -3$, and $c = -5$. By substituting these values into the quadratic formula, we proceed as follows:

$$
x = \frac{-(-3) \pm \sqrt{(-3)^2 - 4(2)(-5)}}{2(2)}.
$$

This simplifies to:

$$
x = \frac{3 \pm \sqrt{9 + 40}}{4}.
$$

Continuing with the simplification, we have:

$$
x = \frac{3 \pm \sqrt{49}}{4}.
$$

Since the square root of $49$ is $7$, we can further simplify to:

$$
x = \frac{3 + 7}{4} \quad \text{or} \quad x = \frac{3 - 7}{4}.
$$

Calculating these two expressions yields:

$$
x = \frac{10}{4} = \frac{5}{2} \quad \text{and} \quad x = \frac{-4}{4} = -1.
$$

Thus, the roots of the quadratic equation 

$$
2x^2 - 3x - 5 = 0 
$$ 

are 

$$
x = \frac{5}{2} \quad \text{and} \quad x = -1.
$$ 

To verify our solutions, we can substitute these values back into the original equation to ensure they satisfy it.
    