---
title: "Prove the half-angle formula for cosine"
summary: The half-angle formula for cosine is $ \cos^2\left(\frac{x}{2}\right) = \frac{1 + \cos(x)}{2} $.
author: "Prof. Sophia Clark"
degree: "PhD in Nuclear Physics, University of Leeds"
tutor_type: "A-Level Maths Tutor"
date: 2024-03-23
---

The half-angle formula for cosine is given by:

$$
\cos^2\left(\frac{x}{2}\right) = \frac{1 + \cos(x)}{2}.
$$

To prove this half-angle formula, we begin with the double-angle formula for cosine:

$$
\cos(2x) = \cos^2(x) - \sin^2(x).
$$

By rearranging this equation, we can express $\cos^2(x)$ in terms of $\cos(2x)$ and $\sin^2(x)$:

$$
\cos^2(x) = \cos(2x) + \sin^2(x).
$$

Next, we substitute $\frac{x}{2}$ for $x$ in the equation above:

$$
\cos^2\left(\frac{x}{2}\right) = \cos(x) + \sin^2\left(\frac{x}{2}\right).
$$

Using the Pythagorean identity, we know that:

$$
\sin^2\left(\frac{x}{2}\right) = \frac{1 - \cos(x)}{2}.
$$

We can now substitute this identity into our equation:

$$
\cos^2\left(\frac{x}{2}\right) = \cos(x) + \frac{1 - \cos(x)}{2}.
$$

To simplify the right-hand side, we combine the terms:

$$
\cos^2\left(\frac{x}{2}\right) = \cos(x) + \frac{1}{2} - \frac{\cos(x)}{2}.
$$

This can be further simplified as follows:

$$
\cos^2\left(\frac{x}{2}\right) = \frac{2\cos(x)}{2} + \frac{1}{2} - \frac{\cos(x)}{2} = \frac{2\cos(x) - \cos(x) + 1}{2} = \frac{\cos(x) + 1}{2}.
$$

Thus, we have derived the half-angle formula for cosine:

$$
\cos^2\left(\frac{x}{2}\right) = \frac{1 + \cos(x)}{2}.
$$

This completes the proof.
    