---
title: "How to integrate csc^2(x)cot^2(x)?"
summary: To integrate $\csc^2(x)\cot^2(x)$, substitute $u = \cot(x)$ to simplify the expression before performing the integration.
author: "Prof. Alan Smith"
degree: "PhD in Physics, University of Cambridge"
tutor_type: "A-Level Physics Tutor"
date: 2024-06-10
---

To integrate the expression \( \csc^2(x) \cot^2(x) \), we can begin by making a substitution. Let's set \( u = \cot(x) \). This choice simplifies the integral significantly.

First, we can utilize the identity \( \cot^2(x) = \csc^2(x) - 1 \) to rewrite the integrand. By substituting this identity, we have:

$$
\csc^2(x) \cot^2(x) = \csc^2(x)(\csc^2(x) - 1) = \csc^4(x) - \csc^2(x).
$$

Next, we differentiate our substitution. The derivative is given by:

$$
\frac{du}{dx} = -\csc^2(x) \quad \Rightarrow \quad dx = -\frac{du}{\csc^2(x)}.
$$

Substituting these expressions into our integral, we obtain:

$$
\int \csc^2(x) \cot^2(x) \, dx = \int (\csc^4(x) - \csc^2(x)) \, dx.
$$

This can be separated into two integrals:

$$
= \int \csc^4(x) \, dx - \int \csc^2(x) \, dx.
$$

Now, substituting \( u = \cot(x) \), we rewrite the integrals as follows:

$$
\int \csc^4(x) \, dx = \int (1 + \cot^2(x))^2 \left(-\frac{du}{\csc^2(x)}\right) - \int \csc^2(x) \, dx.
$$

Since \( \csc^2(x) = 1 + u^2 \), the first integral becomes:

$$
-\int \frac{(u^2 + 2u + 1)}{(1 + u^2)^2} \, du - \int \csc^2(x) \, dx.
$$

Now we can simplify the integrand:

$$
= -\int (u^2 + 2u + 1)(1 + u^2) \, du - \int \csc^2(x) \, dx.
$$

Expanding the polynomial gives:

$$
= -\int (u^4 + 3u^2 + 2u + 1) \, du - \int \csc^2(x) \, dx.
$$

Now we can integrate term by term:

$$
= -\left(\frac{u^5}{5} + u^3 + u + \frac{2u^4}{4} + u^2\right) - \ln |\csc(x) + \cot(x)| + C.
$$

Finally, substituting back \( u = \cot(x) \):

$$
= -\frac{\cot^5(x)}{5} - \cot^3(x) - \cot(x) - \frac{\cot^4(x)}{2} - \cot^2(x) - \ln |\csc(x) + \cot(x)| + C.
$$

Thus, the integral of \( \csc^2(x) \cot^2(x) \) is:

$$
-\frac{\cot^5(x)}{5} - \cot^3(x) - \cot(x) - \frac{\cot^4(x)}{2} - \cot^2(x) - \ln |\csc(x) + \cot(x)| + C.
$$
    