---
title: "Differentiate the function y = ln(x)"
summary: "The derivative of the natural logarithm function y = ln(x) is 1/x, indicating the rate of change of the function with respect to x."
author: "Prof. Peter Brown"
degree: "PhD in Mathematics, University of Warwick"
tutor_type: "IB Maths Tutor"
date: 2024-03-08
---

The derivative of the function \( y = \ln(x) \) is given by 

$$
\frac{dy}{dx} = \frac{1}{x}.
$$

To differentiate \( y = \ln(x) \), we can apply the formula for the derivative of a natural logarithm:

$$
\frac{d}{dx} \ln(x) = \frac{1}{x}.
$$

This indicates that the derivative of \( y = \ln(x) \) equals \( \frac{1}{x} \). To understand why this is the case, we can utilize the definition of the derivative, which is expressed as:

$$
f'(x) = \lim_{h \to 0} \frac{f(x+h) - f(x)}{h}.
$$

Applying this definition to \( y = \ln(x) \), we have:

$$
y' = \lim_{h \to 0} \frac{\ln(x+h) - \ln(x)}{h}.
$$

Using the logarithmic property \( \ln(a) - \ln(b) = \ln\left(\frac{a}{b}\right) \), we can simplify the expression:

$$
y' = \lim_{h \to 0} \frac{\ln\left(\frac{x+h}{x}\right)}{h} = \lim_{h \to 0} \frac{\ln\left(1 + \frac{h}{x}\right)}{h}.
$$

Next, we can rewrite this limit in terms of \( \frac{h}{x} \):

$$
y' = \lim_{h \to 0} \frac{\ln\left(1 + \frac{h}{x}\right)}{\frac{h}{x}} \cdot \frac{1}{x}.
$$

As \( h \) approaches \( 0 \), \( \frac{h}{x} \) also approaches \( 0 \). Using the limit definition of the natural logarithm, we know that 

$$
\ln(1 + u) \approx u \quad \text{as} \quad u \to 0.
$$

Thus,

$$
\lim_{u \to 0} \frac{\ln(1 + u)}{u} = 1.
$$

Applying this to our expression, we find:

$$
y' = 1 \cdot \frac{1}{x} = \frac{1}{x}.
$$

Consequently, we conclude that:

$$
y' = \frac{1}{x}.
$$

This result signifies that the slope of the tangent line to the graph of \( y = \ln(x) \) at any point \( (x, \ln(x)) \) is equal to \( \frac{1}{x} \).
    