---
title: "Find the roots of the quadratic equation x^2 + 5x + 6 = 0"
summary: "The equation x^2 + 5x + 6 = 0 has roots at -2 and -3."
author: "Prof. David Martin"
degree: "PhD in Physics, University of Birmingham"
tutor_type: "A-Level Physics Tutor"
date: 2024-02-08
---

The roots of the quadratic equation $x^2 + 5x + 6 = 0$ are $-2$ and $-3$.

To determine the roots of a quadratic equation in the standard form $ax^2 + bx + c = 0$, we can utilize the quadratic formula:

$$
x = \frac{-b \pm \sqrt{b^2 - 4ac}}{2a}
$$

In this particular case, we have the coefficients $a = 1$, $b = 5$, and $c = 6$. By substituting these values into the quadratic formula, we obtain:

$$
x = \frac{-5 \pm \sqrt{5^2 - 4(1)(6)}}{2(1)}
$$

Next, we simplify the expression under the square root:

$$
x = \frac{-5 \pm \sqrt{25 - 24}}{2}
$$

This simplifies further, as the expression under the square root becomes $1$:

$$
x = \frac{-5 \pm \sqrt{1}}{2}
$$

Since $\sqrt{1} = 1$, we have:

$$
x = \frac{-5 \pm 1}{2}
$$

This results in two potential values for $x$:

1. For the positive case:
   $$
   x = \frac{-5 + 1}{2} = \frac{-4}{2} = -2
   $$

2. For the negative case:
   $$
   x = \frac{-5 - 1}{2} = \frac{-6}{2} = -3
   $$

Thus, the roots of the quadratic equation $x^2 + 5x + 6 = 0$ are indeed $-2$ and $-3$.
    