---
title: "How to find the roots of a quadratic polynomial?"
summary: To find the roots of a quadratic polynomial, apply the quadratic formula $x = \frac{-b \pm \sqrt{b^2 - 4ac}}{2a}$, where $a$, $b$, and $c$ are the coefficients.
author: "Prof. Richard White"
degree: "PhD in Mathematics, University of Leicester"
tutor_type: "A-Level Maths Tutor"
date: 2024-03-21
---

To determine the roots of a quadratic polynomial, we employ the quadratic formula, given by 

$$ 
x = \frac{-b \pm \sqrt{b^2 - 4ac}}{2a}. 
$$

A quadratic polynomial is defined as a polynomial of degree 2, which means its highest exponent of $x$ is 2. It can be expressed in the standard form 

$$ 
ax^2 + bx + c, 
$$ 

where $a$, $b$, and $c$ are constants, and $a \neq 0$. To find the roots of this polynomial, we need to solve the equation when the polynomial equals zero, that is, 

$$ 
ax^2 + bx + c = 0. 
$$

The quadratic formula provides a method for finding the roots of any quadratic polynomial. It is derived from the technique of completing the square on the equation $ax^2 + bx + c = 0$. The formula itself is 

$$ 
x = \frac{-b \pm \sqrt{b^2 - 4ac}}{2a}. 
$$

To utilize the quadratic formula, we substitute the values of $a$, $b$, and $c$ from our specific quadratic polynomial into the formula. Next, we simplify the expression under the square root (the discriminant) and solve for $x$ using both the positive and negative options indicated by the plus/minus sign. If the discriminant, represented as $b^2 - 4ac$, is negative, then the roots are imaginary, indicating that the polynomial does not intersect the $x$-axis.

For instance, let's find the roots of the quadratic polynomial 

$$ 
2x^2 + 5x - 3. 
$$ 

Applying the quadratic formula, we substitute $a = 2$, $b = 5$, and $c = -3$ into the formula:

$$ 
x = \frac{-5 \pm \sqrt{5^2 - 4 \cdot 2 \cdot (-3)}}{2 \cdot 2}. 
$$ 

Simplifying further, we calculate:

$$ 
x = \frac{-5 \pm \sqrt{25 + 24}}{4} = \frac{-5 \pm \sqrt{49}}{4}. 
$$ 

This results in 

$$ 
x = \frac{-5 + 7}{4} \quad \text{and} \quad x = \frac{-5 - 7}{4}, 
$$ 

which simplifies to 

$$ 
x = \frac{1}{2} \quad \text{and} \quad x = -3. 
$$ 

Thus, the roots of the quadratic polynomial $2x^2 + 5x - 3$ are $x = \frac{1}{2}$ and $x = -3$.
    