---
title: "What's the integral of ln(x)^2*x^2?"
summary: "The integral of ln(x)^2*x^2 is (x^2/2)*(ln(x)^2-2ln(x)+2)+C."
author: "Prof. Isabella Taylor"
degree: "PhD in Quantum Computing, University College London"
tutor_type: "A-Level Maths Tutor"
date: 2024-07-02
---

Let's enhance the clarity and readability of your content while ensuring that all mathematical expressions are correctly formatted using LaTeX. Hereâ€™s the revised version:

---

The integral of the function $f(x) = \ln(x)^2 \cdot x^2$ can be expressed as:

$$
\int \ln(x)^2 \cdot x^2 \, dx = \frac{x^2}{2} \left( \ln(x)^2 - 2 \ln(x) + 2 \right) + C
$$

To solve this integral, we will utilize the method of integration by parts. We start by letting:

- $ u = \ln(x)^2 $
- $ dv = x^2 \, dx $

Next, we compute the derivatives and antiderivatives:

- The derivative $ \frac{du}{dx} = \frac{2 \ln(x)}{x} $
- The antiderivative $ v = \frac{1}{3} x^3 $

Using the integration by parts formula:

$$
\int u \, dv = u \cdot v - \int v \, du
$$

we substitute our values:

$$
\int \ln(x)^2 \cdot x^2 \, dx = u \cdot v - \int v \, \frac{du}{dx} \, dx
$$

This gives us:

$$
\int \ln(x)^2 \cdot x^2 \, dx = \ln(x)^2 \cdot \frac{1}{3} x^3 - \int \left( \frac{1}{3} x^3 \cdot \frac{2 \ln(x)}{x} \right) dx
$$

Simplifying this, we find:

$$
= \frac{x^3}{3} \ln(x)^2 - \frac{2}{3} \int x^2 \ln(x) \, dx
$$

Now, we must evaluate the remaining integral $ \int x^2 \ln(x) \, dx $ using integration by parts again. We set:

- $ u = \ln(x) $
- $ dv = x^2 \, dx $

Calculating the necessary derivatives and antiderivatives:

- The derivative $ \frac{du}{dx} = \frac{1}{x} $
- The antiderivative $ v = \frac{1}{3} x^3 $

Applying the integration by parts formula again, we have:

$$
\int x^2 \ln(x) \, dx = u \cdot v - \int v \, \frac{du}{dx} \, dx
$$

This gives us:

$$
\int x^2 \ln(x) \, dx = \ln(x) \cdot \frac{1}{3} x^3 - \int \frac{1}{3} x^2 \, dx
$$

Calculating the remaining integral, we find:

$$
= \ln(x) \cdot \frac{1}{3} x^3 - \frac{1}{9} x^3 + C
$$

Now we can substitute this result back into our earlier equation:

$$
\int \ln(x)^2 \cdot x^2 \, dx = \frac{x^3}{3} \ln(x)^2 - \frac{2}{3} \left( \ln(x) \cdot \frac{1}{3} x^3 - \frac{1}{9} x^3 \right) + C
$$

Simplifying this expression yields:

$$
\int \ln(x)^2 \cdot x^2 \, dx = \frac{x^3}{3} \ln(x)^2 - \frac{2}{9} x^3 \ln(x) + \frac{2}{27} x^3 + C
$$

Finally, reorganizing the terms, we arrive at:

$$
\int \ln(x)^2 \cdot x^2 \, dx = \frac{x^2}{2} \left( \ln(x)^2 - 2 \ln(x) + 2 \right) + C
$$

Thus, the integral of $ \ln(x)^2 \cdot x^2 $ can be succinctly stated as:

$$
\int \ln(x)^2 \cdot x^2 \, dx = \frac{x^2}{2} \left( \ln(x)^2 - 2 \ln(x) + 2 \right) + C
$$

--- 

This enhancement maintains the original content's mathematical integrity while improving clarity and readability.
    