---
title: "Calculate the remainder when x^5 - 4x^4 + 6x^3 - 4x^2 + x - 1 is divided by x - 1"
summary: The polynomial $x^5 - 4x^4 + 6x^3 - 4x^2 + x - 1$ has a remainder of -4 when divided by $x - 1$.
author: "Prof. Peter Brown"
degree: "PhD in Mathematics, University of Warwick"
tutor_type: "IB Maths Tutor"
date: 2024-03-10
---

The remainder when the polynomial \(x^5 - 4x^4 + 6x^3 - 4x^2 + x - 1\) is divided by \(x - 1\) is \(-4\).

To determine the remainder of a polynomial when divided by a linear factor, we can apply the Remainder Theorem. This theorem states that if a polynomial \(f(x)\) is divided by \(x - a\), the remainder is simply \(f(a)\).

In our case, we want to find the remainder when the polynomial \(x^5 - 4x^4 + 6x^3 - 4x^2 + x - 1\) is divided by \(x - 1\). According to the Remainder Theorem, we substitute \(x = 1\) into the polynomial:

$$
f(1) = 1^5 - 4(1)^4 + 6(1)^3 - 4(1)^2 + 1 - 1
$$

Calculating this step-by-step:

1. \(1^5 = 1\)
2. \(-4(1^4) = -4\)
3. \(6(1^3) = 6\)
4. \(-4(1^2) = -4\)
5. \(1 - 1 = 0\)

Now, we combine these results:

$$
f(1) = 1 - 4 + 6 - 4 + 0 = -4
$$

Thus, the remainder when \(x^5 - 4x^4 + 6x^3 - 4x^2 + x - 1\) is divided by \(x - 1\) is indeed \(-4\).
    