---
title: "Explain how to find the nth term of a geometric sequence"
summary: "The nth term of a geometric sequence can be calculated using the formula an = a1 x r^(n-1), where a1 is the first term and r is the common ratio."
author: "Dr. Sarah Wilson"
degree: "MSc in Physics, University College London"
tutor_type: "A-Level Physics Tutor"
date: 2024-01-22
---

To determine the $n$th term of a geometric sequence, we can utilize the following formula:

$$
a_n = a_1 \cdot r^{(n-1)}
$$

In a geometric sequence, each term is derived by multiplying the previous term by a constant known as the common ratio, denoted as $r$. The first term is labeled as $a_1$, the second term as $a_2$, and so forth. To calculate the $n$th term ($a_n$), we apply the formula:

$$
a_n = a_1 \cdot r^{(n-1)}
$$

For instance, consider the geometric sequence: $2, 4, 8, 16, 32, \ldots$ Here, we identify $a_1 = 2$ and $r = 2$. To find the 6th term ($a_6$), we substitute $n = 6$ into the formula:

\[
\begin{align*}
a_6 & = a_1 \cdot r^{(n-1)} \\
& = 2 \cdot 2^{(6-1)} \\
& = 2 \cdot 2^5 \\
& = 2 \cdot 32 \\
& = 64
\end{align*}
\]

Thus, the 6th term of the sequence is $64$.

The behavior of a geometric sequence depends on the value of the common ratio ($r$):

- If $r < 1$, the sequence will converge to zero as $n$ approaches infinity.
- If $r > 1$, the sequence will grow indefinitely as $n$ increases.
- If $r = 1$, the sequence remains constant, as all terms are equal to the first term.
    