---
title: "Find the roots of the quadratic equation x^2 - 5x + 6 = 0"
summary: "The equation x^2 - 5x + 6 = 0 has roots at x = 2 and x = 3."
author: "Dr. Angela Davis"
degree: "MSc in Mathematics, University of Bristol"
tutor_type: "A-Level Maths Tutor"
date: 2024-04-21
---

The roots of the quadratic equation $x^2 - 5x + 6 = 0$ are $x = 2$ and $x = 3$.

To determine the roots of a quadratic equation of the form $ax^2 + bx + c = 0$, we can employ the quadratic formula:

$$
x = \frac{-b \pm \sqrt{b^2 - 4ac}}{2a}
$$

In this specific case, we have $a = 1$, $b = -5$, and $c = 6$. By substituting these values into the quadratic formula, we arrive at the following calculation:

$$
x = \frac{-(-5) \pm \sqrt{(-5)^2 - 4(1)(6)}}{2(1)}
$$

Simplifying this expression step-by-step, we get:

$$
x = \frac{5 \pm \sqrt{25 - 24}}{2}
$$

This reduces to:

$$
x = \frac{5 \pm 1}{2}
$$

Thus, the roots of the equation are $x = 2$ and $x = 3$. 

To verify our results, we can substitute these values back into the original equation:

For $x = 2$:

$$
2^2 - 5(2) + 6 = 0
$$

Calculating this gives:

$$
4 - 10 + 6 = 0 \quad \text{(True)}
$$

For $x = 3$:

$$
3^2 - 5(3) + 6 = 0
$$

Calculating this results in:

$$
9 - 15 + 6 = 0 \quad \text{(True)}
$$

Since both equations hold true, we have successfully confirmed that the roots $x = 2$ and $x = 3$ are indeed correct.
    