---
title: "How to derive the identity for hyperbolic functions?"
summary: "The identity for hyperbolic functions is derived using the definitions of sinh, cosh and tanh."
author: "Dr. Daniel Thompson"
degree: "PhD in Relativity, University of Sheffield"
tutor_type: "A-Level Maths Tutor"
date: 2024-07-08
---

The identity for hyperbolic functions can be derived using the definitions of the hyperbolic sine, cosine, and tangent functions. 

The hyperbolic functions are defined as follows:

$$
\sinh(x) = \frac{e^x - e^{-x}}{2}
$$

$$
\cosh(x) = \frac{e^x + e^{-x}}{2}
$$

$$
\tanh(x) = \frac{\sinh(x)}{\cosh(x)} = \frac{e^x - e^{-x}}{e^x + e^{-x}}
$$

Using these definitions, we can derive the identity:

$$
\cosh^2(x) - \sinh^2(x) = 1
$$

We will start with the left-hand side of the identity:

$$
\cosh^2(x) - \sinh^2(x) = \left( \frac{e^x + e^{-x}}{2} \right)^2 - \left( \frac{e^x - e^{-x}}{2} \right)^2
$$

Expanding both squares, we have:

$$
= \frac{(e^x + e^{-x})^2}{4} - \frac{(e^x - e^{-x})^2}{4}
$$

Calculating each square yields:

$$
= \frac{(e^{2x} + 2 + e^{-2x})}{4} - \frac{(e^{2x} - 2 + e^{-2x})}{4}
$$

Now, simplifying this expression:

$$
= \frac{1}{4} \left( (e^{2x} + 2 + e^{-2x}) - (e^{2x} - 2 + e^{-2x}) \right)
$$

This simplifies to:

$$
= \frac{1}{4} \left( 4 \right) = 1
$$

Thus, we have shown that:

$$
\cosh^2(x) - \sinh^2(x) = 1
$$

This confirms the identity for hyperbolic functions.
    