---
title: "Determine the coefficients of the cubic equation with roots 2, -1, and 1"
summary: "The cubic equation with roots 2, -1, and 1 has coefficients 1, -2, -3, and 2."
author: "Prof. Sophia Clark"
degree: "PhD in Nuclear Physics, University of Leeds"
tutor_type: "A-Level Maths Tutor"
date: 2024-04-27
---

Let's enhance the clarity and readability of the content while ensuring that the mathematical expressions are correctly formatted.

---

The cubic equation with roots $2$, $-1$, and $1$ has coefficients $1$, $-2$, $-3$, and $2$.

To derive the coefficients of a cubic equation from its roots, we begin with the factored form of the equation:

$$(x - r_1)(x - r_2)(x - r_3) = 0$$

where $r_1$, $r_2$, and $r_3$ represent the roots. Expanding this expression results in:

$$x^3 - (r_1 + r_2 + r_3)x^2 + (r_1r_2 + r_1r_3 + r_2r_3)x - r_1r_2r_3 = 0$$

By comparing this expanded form to the standard representation of a cubic equation:

$$ax^3 + bx^2 + cx + d = 0$$

we can establish the relationships between the coefficients and the roots as follows:

- $a = 1$
- $b = -(r_1 + r_2 + r_3)$
- $c = r_1r_2 + r_1r_3 + r_2r_3$
- $d = -r_1r_2r_3$

Now, substituting the given roots into these formulas, we find:

- $a = 1$
- $b = -(2 + (-1) + 1) = -2$
- $c = 2 \cdot (-1) \cdot 1 + 2 \cdot 2 \cdot 1 + (-1) \cdot 1 = -2$
- $d = -(2 \cdot (-1) \cdot 1) = 2$

Thus, the coefficients of the cubic equation with roots $2$, $-1$, and $1$ are $1$, $-2$, $-2$, and $2$. The final equation can be expressed as:

$$x^3 - 2x^2 - 2x + 2 = 0$$

This provides a clear and structured understanding of the relationship between the roots and the coefficients of the cubic equation.
    