---
title: "Calculate the derivative of the function y = ln(x)"
summary: "The derivative of the natural logarithm function, y = ln(x), is 1/x, indicating the rate of change of the function with respect to x."
author: "Prof. David Martin"
degree: "PhD in Physics, University of Birmingham"
tutor_type: "A-Level Physics Tutor"
date: 2024-07-15
---

To find the derivative of the function \( y = \ln(x) \), we start by applying the known formula for the derivative of a natural logarithm:

$$
\frac{d}{dx} \ln(x) = \frac{1}{x}.
$$

This formula indicates that the derivative of \( \ln(x) \) is equal to \( \frac{1}{x} \). We can demonstrate this result using the definition of the derivative:

$$
\lim_{h \to 0} \frac{\ln(x+h) - \ln(x)}{h}.
$$

We can simplify this expression as follows:

$$
= \lim_{h \to 0} \frac{\ln\left(\frac{x+h}{x}\right)}{h} 
= \lim_{h \to 0} \frac{\ln\left(1 + \frac{h}{x}\right)}{h}.
$$

Next, we can factor out \( \frac{1}{x} \) from the limit:

$$
= \lim_{h \to 0} \left(\frac{1}{x} \cdot \frac{\ln\left(1 + \frac{h}{x}\right)}{h}\right) 
= \frac{1}{x} \lim_{h \to 0} \frac{\ln\left(1 + \frac{h}{x}\right)}{h}.
$$

To evaluate the limit inside the parentheses, we can apply L'Hôpital's Rule, as both the numerator and denominator approach \( 0 \) as \( h \) approaches \( 0 \):

$$
\lim_{h \to 0} \frac{\ln\left(1 + \frac{h}{x}\right)}{h}.
$$

Applying L'Hôpital's Rule yields:

$$
= \lim_{h \to 0} \frac{\frac{1}{1 + \frac{h}{x}} \cdot \frac{1}{x}}{1} 
= \frac{1}{x} \lim_{h \to 0} \frac{1}{1 + \frac{h}{x}} 
= \frac{1}{x} \cdot 1 
= \frac{1}{x}.
$$

Therefore, we conclude that the derivative of \( y = \ln(x) \) is indeed 

$$
\frac{1}{x}.
$$
    