---
title: "Find the roots of the quadratic equation 3x^2 - 4x + 1 = 0"
summary: "The quadratic equation 3x^2 - 4x + 1 = 0 has roots at 1/3 and 1."
author: "Prof. Peter Brown"
degree: "PhD in Mathematics, University of Warwick"
tutor_type: "IB Maths Tutor"
date: 2024-05-18
---

The roots of the quadratic equation 

$$ 
3x^2 - 4x + 1 = 0 
$$ 

are \( \frac{1}{3} \) and \( 1 \).

To determine the roots of a quadratic equation in the standard form \( ax^2 + bx + c = 0 \), we can utilize the quadratic formula:

$$ 
x = \frac{-b \pm \sqrt{b^2 - 4ac}}{2a} 
$$ 

In our equation, we have \( a = 3 \), \( b = -4 \), and \( c = 1 \). Substituting these values into the formula gives us:

$$ 
x = \frac{-(-4) \pm \sqrt{(-4)^2 - 4(3)(1)}}{2(3)} 
$$ 

Calculating step-by-step:

1. Simplify the expression:
$$ 
x = \frac{4 \pm \sqrt{16 - 12}}{6} 
$$ 

2. Continue simplifying under the square root:
$$ 
x = \frac{4 \pm \sqrt{4}}{6} 
$$ 

3. Calculate the square root:
$$ 
x = \frac{4 \pm 2}{6} 
$$ 

This results in two possible values for \( x \):

1. When we take the positive root:
$$ 
x = \frac{4 + 2}{6} = \frac{6}{6} = 1 
$$ 

2. When we take the negative root:
$$ 
x = \frac{4 - 2}{6} = \frac{2}{6} = \frac{1}{3} 
$$ 

Thus, the roots of the equation are \( \frac{1}{3} \) and \( 1 \). 

To verify these roots, we can substitute them back into the original equation:

1. Checking \( x = \frac{1}{3} \):
$$ 
3\left(\frac{1}{3}\right)^2 - 4\left(\frac{1}{3}\right) + 1 = 0 
$$ 
Simplifying this gives:
$$ 
3 \cdot \frac{1}{9} - \frac{4}{3} + 1 = 0 
$$ 
$$ 
\frac{1}{3} - \frac{4}{3} + \frac{3}{3} = 0 
$$ 
$$ 
\frac{1 - 4 + 3}{3} = 0 
$$ 
This simplifies to:
$$ 
\frac{0}{3} = 0 
$$ 

2. Checking \( x = 1 \):
$$ 
3(1)^2 - 4(1) + 1 = 0 
$$ 
This simplifies to:
$$ 
3 - 4 + 1 = 0 
$$ 
Which is:
$$ 
0 = 0 
$$ 

Both roots satisfy the original quadratic equation, confirming that our calculations are correct.
    