---
title: "How to integrate csc^2(x)cot^3(x)?"
summary: "To integrate csc^2(x)cot^3(x), use u-substitution with u = cot(x) and du = -csc^2(x)dx."
author: "Dr. Daniel Thompson"
degree: "PhD in Relativity, University of Sheffield"
tutor_type: "A-Level Maths Tutor"
date: 2024-07-16
---

To integrate the expression $ \csc^2(x) \cot^3(x) $, we can utilize u-substitution. We start by setting $ u = \cot(x) $. Consequently, the differential $ du $ can be expressed as $ du = -\csc^2(x) \, dx $.

With this substitution, the integral transforms as follows:

$$
\int \csc^2(x) \cot^3(x) \, dx = \int -u^3 \, du.
$$

Now, we proceed by integrating $ -u^3 $:

$$
\int -u^3 \, du = -\frac{1}{4} u^4 + C,
$$

where $ C $ is the constant of integration.

Next, we substitute back for $ u $:

$$
-\frac{1}{4} u^4 + C = -\frac{1}{4} \cot^4(x) + C.
$$

Thus, the final result for the integral is:

$$
\int \csc^2(x) \cot^3(x) \, dx = -\frac{1}{4} \cot^4(x) + C.
$$
    