---
title: "Find the roots of the quadratic equation 2x^2 + 3x + 1 = 0"
summary: "The roots of the quadratic equation 2x^2 + 3x + 1 = 0 are -1 and -0.5."
author: "Prof. Sophia Clark"
degree: "PhD in Nuclear Physics, University of Leeds"
tutor_type: "A-Level Maths Tutor"
date: 2024-04-19
---

The roots of the quadratic equation $$2x^2 + 3x + 1 = 0$$ are $-1$ and $-0.5$.

To determine the roots of a quadratic equation, we can utilize the quadratic formula:

$$ x = \frac{-b \pm \sqrt{b^2 - 4ac}}{2a} $$

In this formula, $a$, $b$, and $c$ represent the coefficients of the quadratic equation in the standard form $$ax^2 + bx + c = 0$$.

For the given equation, we have $a = 2$, $b = 3$, and $c = 1$. Plugging these values into the quadratic formula yields:

$$ x = \frac{-3 \pm \sqrt{3^2 - 4(2)(1)}}{2(2)} $$

Calculating the discriminant:

$$ x = \frac{-3 \pm \sqrt{9 - 8}}{4} $$
$$ x = \frac{-3 \pm \sqrt{1}}{4} $$

Now, simplifying further, we find:

$$ x = \frac{-3 + 1}{4} \quad \text{or} \quad x = \frac{-3 - 1}{4} $$
$$ x = \frac{-2}{4} \quad \text{or} \quad x = \frac{-4}{4} $$
$$ x = -0.5 \quad \text{or} \quad x = -1 $$

Thus, the roots of the quadratic equation $$2x^2 + 3x + 1 = 0$$ are indeed $-1$ and $-0.5$. 

To confirm our results, we can substitute these values back into the original equation and verify that they satisfy the equation.
    