---
title: "How to solve a cubic equation?"
summary: To solve a cubic equation, use the formula $x = \frac{-b \pm \sqrt{b^2 - 4ac + 3a^2}}{3a}$.
author: "Prof. Sophia Clark"
degree: "PhD in Nuclear Physics, University of Leeds"
tutor_type: "A-Level Maths Tutor"
date: 2024-09-09
---

To solve a cubic equation, begin by ensuring it is expressed in the standard form:

$$
ax^3 + bx^2 + cx + d = 0.
$$

Once in this format, you can apply the following formula to find the roots:

$$
x = \frac{-b \pm \sqrt{b^2 - 4ac + 3a^2}}{3a}.
$$

This formula is derived from the quadratic formula and is applicable for determining the roots of any cubic equation.

### Example: Solving a Specific Cubic Equation

Consider the cubic equation:

$$
x^3 - 6x^2 + 11x - 6 = 0.
$$

First, we identify the coefficients: $a = 1$, $b = -6$, $c = 11$, and $d = -6$. Substituting these values into the formula gives us:

$$
x = \frac{-(-6) \pm \sqrt{(-6)^2 - 4(1)(11) + 3(1)^2}}{3(1)}.
$$

Now, simplifying the expression step by step:

1. Compute $(-6)^2 = 36$.
2. Calculate $4(1)(11) = 44$.
3. Find $3(1)^2 = 3$.

Thus, we rewrite the expression:

$$
x = \frac{6 \pm \sqrt{36 - 44 + 3}}{3}.
$$

This simplifies further:

$$
x = \frac{6 \pm \sqrt{-5}}{3}.
$$

Since the square root of a negative number is not a real number, we conclude that this cubic equation has no real roots.

### Complex Roots in Cubic Equations

When a cubic equation has complex roots, those roots typically appear in conjugate pairs. As an illustration, consider the equation:

$$
x^3 + 3x^2 + 3x + 1 = 0.
$$

The roots of this equation include $-1$, $-1 + i$, and $-1 - i$. To find these roots, we again use the same formula, substituting $a = 1$, $b = 3$, $c = 3$, and $d = 1$:

$$
x = \frac{-3 \pm \sqrt{3^2 - 4(1)(3) + 3(1)^2}}{3}.
$$

Calculating the terms inside the square root:

1. Compute $3^2 = 9$.
2. Calculate $4(1)(3) = 12$.
3. Find $3(1)^2 = 3$.

This leads us to:

$$
x = \frac{-3 \pm \sqrt{9 - 12 + 3}}{3} = \frac{-3 \pm \sqrt{0}}{3}.
$$

This simplifies to:

$$
x = \frac{-3}{3} = -1.
$$

Next, we can factor the original cubic equation. By using long division or synthetic division, we can factor out $(x + 1)^2$, which leaves us with:

$$
(x + 1)^2 (x + 1 - i)(x + 1 + i) = 0.
$$

Thus, the roots of the equation are:

$$
-1, \quad -1 + i, \quad -1 - i.
$$

These steps demonstrate how to solve cubic equations, both with real roots and complex roots.
    