---
title: "How to derive the identity for hyperbolic sine?"
summary: "To derive the identity for hyperbolic sine, use the definition sinh(x) = (e^x - e^(-x))/2, and explore its properties and relationships with exponential functions for further insights."
author: "Dr. Emily Clark"
degree: "PhD in Mathematics, University of Edinburgh"
tutor_type: "A-Level Maths Tutor"
date: 2024-07-15
---

### Deriving the Identity for Hyperbolic Sine

The identity for the hyperbolic sine function, denoted as $\sinh(x)$, is derived using the properties of the exponential function.

The hyperbolic sine function is defined as:

$$
\sinh(x) = \frac{e^x - e^{-x}}{2}
$$

To derive the identity, we start with the definition of $\sinh(x)$ and multiply both the numerator and denominator by $e^x$:

$$
\sinh(x) = \frac{e^x - e^{-x}}{2} \cdot \frac{e^x}{e^x} = \frac{e^{2x} - 1}{2e^x}
$$

Next, we utilize the identity $e^{2x} = (e^x)^2$ to rewrite the numerator:

$$
\sinh(x) = \frac{(e^x)^2 - 1}{2e^x}
$$

This expression can be factored as follows:

$$
\sinh(x) = \frac{(e^x - 1)(e^x + 1)}{2e^x}
$$

We can further rearrange the terms:

$$
\sinh(x) = \frac{e^x/2 - e^{-x}/2}{e^x/2 + e^{-x}/2}
$$

Next, we apply the difference of squares formula:

$$
\sinh(x) = \left( \frac{e^x}{2} \right)^2 - \left( \frac{e^{-x}}{2} \right)^2
$$

This can be expressed as:

$$
\sinh(x) = \frac{(e^x)^2 - (1)^2}{4} = \frac{e^{2x} - 1}{4}
$$

Continuing with simplification, we find:

$$
\sinh(x) = 1 - \frac{e^x}{2} \left(1 - \frac{e^x}{2}\right) = 1 - \frac{(1 - e^x)}{2}
$$

Thus, we can conclude with:

$$
\sinh(x) = \frac{e^x}{2}
$$

In summary, we have derived the identity for hyperbolic sine:

$$
\sinh(x) = \frac{e^x - e^{-x}}{2} = \frac{e^x}{2} - \frac{e^{-x}}{2} = \frac{e^x - 1}{2e^{-x}}
$$

This demonstrates the various forms of the hyperbolic sine identity.
    