---
title: "How do you determine the equation of a line perpendicular to y = 4x + 1?"
summary: To find a line perpendicular to $ y = 4x + 1 $, calculate the negative reciprocal of the slope (4), resulting in a new slope of $-\frac{1}{4}$.
author: "Prof. Michael Lewis"
degree: "PhD in Physics, University of Oxford"
tutor_type: "IB Physics Tutor"
date: 2024-07-10
---

To find the equation of a line that is perpendicular to the line given by $ y = 4x + 1 $, we begin by determining the slope of the original line and then using its negative reciprocal.

The slope (or gradient) of the line $ y = 4x + 1 $ is $ 4 $. For a line to be perpendicular to this one, its slope must be the negative reciprocal of $ 4 $. The negative reciprocal of $ 4 $ is $ -\frac{1}{4} $. Thus, the slope of the perpendicular line will be $ -\frac{1}{4} $.

Next, we will employ the point-slope form of the line equation, which is expressed as 

$$ y - y_1 = m(x - x_1) $$ 

where $ m $ denotes the slope and $(x_1, y_1)$ represents a point on the line. If you have a specific point through which the perpendicular line passes, you can substitute that point along with the slope $ -\frac{1}{4} $ into this equation.

For instance, if the perpendicular line passes through the point $(2, 3)$, we substitute $ m = -\frac{1}{4} $, $ x_1 = 2 $, and $ y_1 = 3 $ into the point-slope form:

$$ y - 3 = -\frac{1}{4}(x - 2) $$

Now, let's simplify this equation to convert it into slope-intercept form, $ y = mx + c $:

Starting with:

$$ y - 3 = -\frac{1}{4} (x - 2) $$

Expanding the right side gives:

$$ y - 3 = -\frac{1}{4}x + \frac{1}{2} $$

Next, we add $ 3 $ to both sides:

$$ y = -\frac{1}{4}x + \frac{1}{2} + 3 $$

To combine the constants, we convert $ 3 $ into a fraction:

$$ y = -\frac{1}{4}x + \frac{1}{2} + \frac{6}{2} $$

This simplifies to:

$$ y = -\frac{1}{4}x + \frac{7}{2} $$

Therefore, the equation of the line that is perpendicular to $ y = 4x + 1 $ and passes through the point $(2, 3)$ is 

$$ y = -\frac{1}{4}x + \frac{7}{2} $$.
    