---
title: "What is the inverse of f(x) = 3x - 4?"
summary: The inverse function of $ f(x) = 3x - 4 $ is $ f^{-1}(x) = \frac{x + 4}{3} $.
author: "Prof. David Martin"
degree: "PhD in Physics, University of Birmingham"
tutor_type: "A-Level Physics Tutor"
date: 2024-07-22
---

The inverse of the function $ f(x) = 3x - 4 $ is given by 

$$ 
f^{-1}(x) = \frac{x + 4}{3}. 
$$

To find the inverse of a function, we need to interchange the roles of $ x $ and $ y $ and then solve for $ y $. Let's begin with the original function $ f(x) = 3x - 4 $. We start by substituting $ f(x) $ with $ y $, which gives us the equation:

$$ 
y = 3x - 4. 
$$

Next, we swap $ x $ and $ y $ to obtain:

$$ 
x = 3y - 4. 
$$

Our objective now is to solve this equation for $ y $. We begin by adding 4 to both sides to isolate the term containing $ y $:

$$ 
x + 4 = 3y. 
$$

Now, we divide both sides by 3 to isolate $ y $:

$$ 
y = \frac{x + 4}{3}. 
$$

Thus, the inverse function $ f^{-1}(x) $ is 

$$ 
f^{-1}(x) = \frac{x + 4}{3}. 
$$

In simpler terms, the inverse function effectively "reverses" the operations performed by the original function. Specifically, if the original function takes an input $ x $, multiplies it by 3, and then subtracts 4, the inverse function will take an input, add 4, and then divide by 3 to retrieve the original $ x $. This concept is fundamental in various areas of mathematics, as it aids in understanding how functions can be reversed or undone.
    