---
title: "How do you write the equation of a line perpendicular to y = x + 3?"
summary: The equation of a line perpendicular to $ y = x + 3 $ has the form $ y = -x + c $.
author: "Prof. Peter Brown"
degree: "PhD in Mathematics, University of Warwick"
tutor_type: "IB Maths Tutor"
date: 2024-04-08
---

The equation of a line that is perpendicular to the line given by $ y = x + 3 $ can be expressed in the form $ y = -x + c $.

To understand this, we first examine the slope of the original line $ y = x + 3 $. In this equation, the coefficient of $ x $ is $ 1 $, which indicates that the slope of this line is $ 1 $. When two lines are perpendicular, the product of their slopes is $ -1 $. Consequently, if one line has a slope of $ 1 $, the slope of the line that is perpendicular to it must be $ -1 $.

Next, we need to formulate the equation of a line with a slope of $ -1 $. The general form of a linear equation is given by 

$$
y = mx + c,
$$ 

where $ m $ represents the slope and $ c $ denotes the y-intercept. Since we are interested in a perpendicular line with a slope $ m = -1 $, the equation simplifies to 

$$
y = -x + c.
$$

The value of $ c $ can be any real number, which determines where the line intersects the y-axis. For instance, if the line intersects the y-axis at $ 2 $, the equation would be 

$$
y = -x + 2.
$$ 

Conversely, if it intersects at $ -4 $, the equation would take the form 

$$
y = -x - 4.
$$

In summary, the critical insight is that the slope of the perpendicular line is the negative reciprocal of the slope of the original line. For the line $ y = x + 3 $, this means that the perpendicular line will indeed have a slope of $ -1 $, resulting in the general equation 

$$
y = -x + c.
$$
    