---
title: "How do you calculate (2^3)^2?"
summary: To calculate $(2^3)^2$, you multiply the exponents to get $2^{3 \times 2} = 2^6 = 64$.
author: "Dr. Emily Clark"
degree: "PhD in Mathematics, University of Edinburgh"
tutor_type: "GCSE Maths Tutor"
date: 2024-05-29
---

To evaluate the expression $(2^3)^2$, we will apply the laws of exponents, specifically the rule that states when you raise a power to another power, you multiply the exponents. 

In this case, the base is $2$, the first exponent is $3$, and the second exponent is $2$. Therefore, we can rewrite the expression as follows:

$$
(2^3)^2 = 2^{3 \times 2} = 2^6.
$$

Next, we need to calculate $2^6$. This involves multiplying $2$ by itself a total of $6$ times:

$$
2^6 = 2 \times 2 \times 2 \times 2 \times 2 \times 2.
$$

Letâ€™s break this calculation down step by step for clarity:

1. $2 \times 2 = 4$
2. $4 \times 2 = 8$
3. $8 \times 2 = 16$
4. $16 \times 2 = 32$
5. $32 \times 2 = 64$

Thus, we find that $2^6 = 64$. Consequently, we conclude that:

$$
(2^3)^2 = 64.
$$

This method can be applied to any similar problem involving a power raised to another power. Just remember to multiply the exponents first, and then compute the resulting power.
    