---
title: How do you find $(f \circ g)(x)$ for $f(x) = x^2$ and $g(x) = x - 1$?
summary: To find $(f \circ g)(x)$, substitute $g(x)$ into $f(x)$, resulting in $(x - 1)^2$.
author: "Prof. David Martin"
degree: "PhD in Physics, University of Birmingham"
tutor_type: "A-Level Physics Tutor"
date: 2024-08-01
---

To determine the composite function $(f \circ g)(x)$, we begin by substituting $g(x)$ into $f(x)$, which results in the expression $(x - 1)^2$.

To clarify, the notation $(f \circ g)(x)$ indicates that we first apply the function $g(x)$ and then apply the function $f(x)$ to the outcome. Here, we define the functions as follows: $f(x) = x^2$ and $g(x) = x - 1$. The process to find $(f \circ g)(x)$ involves replacing $x$ in $f(x)$ with $g(x)$.

First, we identify $g(x)$:
$$
g(x) = x - 1.
$$
This means that we will substitute $x - 1$ in place of $x$ in the function $f(x)$.

Next, we take the expression for $f(x)$, which is $x^2$, and substitute $x - 1$ for $x$. Consequently, we have:
$$
f(g(x)) = f(x - 1) = (x - 1)^2.
$$

Now, letâ€™s expand $(x - 1)^2$ to further simplify the expression:
$$
(x - 1)^2 = (x - 1)(x - 1) = x^2 - 2x + 1.
$$

Thus, we arrive at the final result for the composite function:
$$
(f \circ g)(x) = (x - 1)^2 = x^2 - 2x + 1.
$$

In conclusion, the composite function $(f \circ g)(x)$ simplifies to $x^2 - 2x + 1$. Understanding how to substitute one function into another is crucial for mastering the concept of composite functions.
    